DS/RedBlack.v
@@ -25,16 +25,25 @@ Inductive elem {A : Type} (x : A) : RBTree A -> Prop :=
     | elem_right : forall  (c : color) (v : A) (l r : RBTree A),
         elem x r -> elem x (T c l v r).
 
-Hint Constructors color RBTree elem.
+Inductive isBST {A : LinDec} : RBTree A -> Prop :=
+    | isBST_E : isBST E
+    | isBST_T : forall (c : color) (v : A) (l r : RBTree A),
+        (forall x : A, elem x l -> leq x v) -> isBST l ->
+        (forall x : A, elem x r -> leq v x) -> isBST r ->
+        isBST (T c l v r).
 
-Ltac inv H := inversion H; clear H; subst; cbn; auto.
+Hint Constructors color RBTree elem isBST.
 
-Lemma elem_color :
-  forall (A : Type) (c c' : color) (x v : A) (l r : RBTree A),
-    elem x (T c l v r) -> elem x (T c' l v r).
-Proof.
-  intros; inv H.
-Qed.
+(** [empty], [isEmpty] and [singleton] are my own. *)
+Definition empty {A : Type} : RBTree A := E.
+
+Definition isEmpty {A : Type} (t : RBTree A) : bool :=
+match t with
+    | E => true
+    | _ => false
+end.
+
+Definition singleton {A : Type} (x : A) : RBTree A := T Red E x E.
 
 Function balance {A : Type} (c : color)
   (l : RBTree A) (v : A) (r : RBTree A) : RBTree A :=
@@ -57,17 +66,6 @@ match t with
     | T _ l v r => T Black l v r
 end.
 
-(*Function ins {A : LinDec} (x : A) (t : RBTree A) : RBTree A :=
-match t with
-    | E => T Red E x E
-    | T c l v r =>
-        if x <=? v
-        then balance c (ins x l) v r
-        else if v <=? x
-          then balance c l v (ins x r)
-          else T c l x r
-end.*)
-
 Function ins {A : LinDec} (x : A) (t : RBTree A) : RBTree A :=
 match t with
     | E => T Red E x E
@@ -80,83 +78,306 @@ end.
 Definition insert {A : LinDec} (x : A) (t : RBTree A) : RBTree A :=
   makeBlack (ins x t).
 
-Require Import Coq.Logic.FunctionalExtensionality.
+Fixpoint count_RBT {A : LinDec} (x : A) (t : RBTree A) : nat :=
+match t with
+    | E => 0
+    | T _ l v r =>
+        (if x =? v then S else id) (count_RBT x l + count_RBT x r)
+end.
 
-Lemma T_not_E :
-  forall (A : Type) (c : color) (v : A) (l r : RBTree A),
-    T c l v r <> E.
-Proof.
-  inversion 1.
-Qed.
+Function toList {A : Type} (t : RBTree A) : list A :=
+match t with
+    | E => []
+    | T _ l v r => toList l ++ v :: toList r
+end.
 
-Lemma balance_not_E :
-  forall (A : Type) (c : color) (v : A) (l r : RBTree A),
-    balance c l v r <> E.
-Proof.
-  intros. functional induction @balance A c l v r; apply T_not_E.
-Qed.
+Fixpoint fromList {A : LinDec} (l : list A) : RBTree A :=
+match l with
+    | [] => E
+    | h :: t => insert h (fromList t)
+end.
 
-Lemma balance_is_T :
-  forall (A : Type) (c : color) (v : A) (l r : RBTree A),
-    exists (c' : color) (v' : A) (l' r' : RBTree A),
-      balance c l v r = T c' l' v' r'.
-Proof.
-  intros. functional induction @balance A c l v r; eauto 6.
-Qed.
+Definition redblackSort (A : LinDec) (l : list A) : list A :=
+  toList (fromList l).
 
-(*Ltac dst := repeat
-match goal with
-    | |- context [if ?x then _ else _] => destruct x
-    | |- context [match ?x with _ => _ end] => destruct x
-end; try apply T_not_E.*)
+(*Definition redblackSort' (A : LinDec) (l : list A) : list A :=
+  toList' (fromList' l).*)
 
-Lemma ins_not_E :
-  forall (A : LinDec) (x : A) (t : RBTree A),
-    ins x t <> E.
-Proof.
-  intros. functional induction @ins A x t;
-  try apply T_not_E; apply balance_not_E.
-Qed.
+(** Properties of [isEmpty]. *)
 
-Inductive is_bst {A : LinDec} : RBTree A -> Prop :=
-    | is_bst_E : is_bst E
-    | is_bst_T : forall (c : color) (v : A) (l r : RBTree A),
-        (forall x : A, elem x l -> leq x v) -> is_bst l ->
-        (forall x : A, elem x r -> leq v x) -> is_bst r ->
-        is_bst (T c l v r).
-
-Hint Constructors is_bst.
-
-Lemma color_is_bst :
-  forall (A : LinDec) (c c' : color) (v : A) (l r : RBTree A),
-    is_bst (T c l v r) <-> is_bst (T c' l v r).
-Proof.
-  split; intros; inv H.
-Qed.
-
-Hint Resolve elem_color.
-
-(*Lemma balance_is_bst :
+Lemma isEmpty_balance :
   forall (A : LinDec) (c : color) (v : A) (l r : RBTree A),
-    is_bst (T c l v r) -> is_bst (balance c l v r).
+    isEmpty (balance c l v r) = false.
 Proof.
   intros. functional induction @balance (@carrier A) c l v r;
-  try assumption.
-    inv H. inv H5. inv H8. constructor; intros; auto.
-      apply H3. eapply elem_color. eauto.
-      inv H.
-      apply H3.
-      apply *)
+  cbn; reflexivity.
+Qed.
 
-(*Ltac bd := intros; repeat (match goal with
-    | |- context [if ?x then _ else _] =>
-        bdestruct (x); subst; cbn in *; try discriminate; auto
-    | H : (?x <? ?y) = _ |- _ => destruct (blt_reflect x y); try congruence
-    | H : ?x <> ?x |- _ => contradiction
-    | H : ?x = ?x |- _ => clear H
-    | H : ~ ?x < ?y, H' : ~ ?y < ?x |- _ =>
-        assert (x = y) by (unfold key in *; omega); subst; clear H; clear H'
-    | H : Abs E _ |- _ => inv H    
-    | H : Abs (T _ _ _ _ _) _ |- _ => inv H
-    | _ => auto; omega
-end; st; cbn in *)
+Lemma isEmpty_makeBlack :
+  forall (A : LinDec) (t : RBTree A),
+    isEmpty (makeBlack t) = isEmpty t.
+Proof.
+  destruct t; cbn; reflexivity.
+Qed.
+
+Lemma isEmpty_ins :
+  forall (A : LinDec) (x : A) (t : RBTree A),
+    isEmpty (ins x t) = false.
+Proof.
+  intros. functional induction @ins A x t;
+  cbn; rewrite ?isEmpty_balance; reflexivity.
+Qed.
+
+Lemma isEmpty_insert :
+  forall (A : LinDec) (x : A) (t : RBTree A),
+    isEmpty (insert x t) = false.
+Proof.
+  intros. unfold insert. rewrite isEmpty_makeBlack, isEmpty_ins. reflexivity.
+Qed.
+
+(** Properties of [singleton]. *)
+
+Lemma singleton_elem :
+  forall (A : LinDec) (x y : A),
+    elem x (singleton y) <-> x = y.
+Proof.
+  unfold singleton. split.
+    inv 1; inv H1.
+    intros ->. auto.
+Qed.
+
+Lemma singleton_isBST :
+  forall (A : LinDec) (x : A),
+    isBST (singleton x).
+Proof.
+  unfold singleton. intros. constructor; auto; inv 1.
+Qed.
+
+(** Properties of [balance]. *)
+
+Lemma elem_inv :
+  forall (A : Type) (P : A -> Prop) (c : color) (v : A) (l r : RBTree A),
+    (forall x : A, elem x (T c l v r) -> P x) ->
+      P v /\
+      (forall x : A, elem x l -> P x) /\
+      (forall x : A, elem x r -> P x).
+Proof.
+  repeat split; intros; apply H; auto.
+Qed.
+
+Ltac aux := intros;
+repeat match goal with
+    | H : context [match ?x with _ => _ end] |- _ => destruct x
+end; cbn in *;
+try match goal with
+    | H : False |- _ => destruct H
+end;
+repeat match goal with
+    | H : isBST (T _ _ _ _) |- _ => inv H
+    | H : elem _ E |- _ => destruct H
+    | H : elem _ (T _ _ _ _) |- _ => inv H
+    | |- isBST _ => constructor; auto
+    | |- forall _, elem _ _ -> _ => inv 1
+end;
+repeat match goal with
+    | H : _ /\ _ |- _ => destruct H
+    | H : forall _, elem _ (T _ _ _ _) -> _ |- _ =>
+        apply elem_inv in H
+end;
+repeat match goal with
+    | H : forall _, elem _ _ -> _, H' : elem _ _ |- _ =>
+        specialize (H _ H')
+end;
+try match goal with
+    | H : ?a ≤ ?b |- ?a ≤ ?b => assumption
+    | H : ?a ≤ ?b, H' : ?b≤ ?c |- ?a ≤ ?c =>
+        apply leq_trans with b; assumption
+end.
+
+Lemma balance_elem :
+  forall (A : LinDec) (c : color) (x v : A) (l r : RBTree A),
+    elem x (T c l v r) <-> elem x (balance c l v r).
+Proof.
+  Time split; functional induction @balance (@carrier A) c l v r; aux.
+Qed.
+
+Lemma balance_isBST :
+  forall (A : LinDec) (c : color) (v : A) (l r : RBTree A),
+    isBST (T c l v r) -> isBST (balance c l v r).
+Proof.
+  Time intros; functional induction @balance (@carrier A) c l v r; aux.
+Qed.
+
+Lemma balance_count_RBT :
+  forall (A : LinDec) (c : color) (x v : A) (l r : RBTree A),
+    count_RBT x (balance c l v r) = count_RBT x (T c l v r).
+Proof.
+  intros. functional induction @balance (@carrier A) c l v r;
+  cbn; dec; unfold id; omega.
+Qed.
+
+(** Properties of [makeBlack]. *)
+
+Lemma makeBlack_elem :
+  forall (A : LinDec) (x : A) (t : RBTree A),
+    elem x (makeBlack t) <-> elem x t.
+Proof.
+  split; destruct t; cbn; auto; inv 1.
+Qed.
+
+Lemma makeBlack_isBST :
+  forall (A : LinDec) (t : RBTree A),
+    isBST t -> isBST (makeBlack t).
+Proof.
+  destruct t; cbn; inv 1.
+Qed.
+
+Lemma makeBlack_count_RBT :
+  forall (A : LinDec) (x : A) (t : RBTree A),
+    count_RBT x (makeBlack t) = count_RBT x t.
+Proof.
+  destruct t; auto.
+Qed.
+
+(** Properties of [ins]. *)
+
+Lemma ins_elem :
+  forall (A : LinDec) (x y : A) (t : RBTree A),
+    elem x (ins y t) <-> x = y \/ elem x t.
+Proof.
+  split.
+    induction t; cbn; intros.
+      inv H.
+      dec; rewrite <- balance_elem in H; inv H; firstorder.
+    induction t; cbn; intros.
+      inv H.
+      dec; rewrite <- balance_elem; inv H; inv H0.
+Qed.
+
+Lemma ins_isBST :
+  forall (A : LinDec) (x : A) (t : RBTree A),
+    isBST t -> isBST (ins x t).
+Proof.
+  intros. functional induction ins x t.
+    constructor; auto; inv 1.
+    apply balance_isBST. inv H. constructor; auto.
+      intros. rewrite ins_elem in H. destruct H; subst; dec.
+    apply balance_isBST. inv H. constructor; auto.
+      intros. rewrite ins_elem in H. destruct H; subst; dec.
+Qed.
+
+Lemma ins_count_RBT :
+  forall (A : LinDec) (x y : A) (t : RBTree A),
+    count_RBT x (ins y t) = (if x =? y then S else id) (count_RBT x t).
+Proof.
+  induction t; cbn; dec;
+  rewrite balance_count_RBT; cbn; rewrite ?IHt1, ?IHt2; dec.
+    unfold id. rewrite plus_n_Sm. reflexivity.
+Qed.
+
+(** Properties of [insert]. *)
+
+Lemma insert_elem :
+  forall (A : LinDec) (x y : A) (t : RBTree A),
+    elem x (insert y t) <-> x = y \/ elem x t.
+Proof.
+  unfold insert. intros. rewrite makeBlack_elem, ins_elem. reflexivity.
+Qed.
+
+Lemma insert_isBST :
+  forall (A : LinDec) (x : A) (t : RBTree A),
+    isBST t -> isBST (insert x t).
+Proof.
+  intros. unfold insert. apply makeBlack_isBST, ins_isBST. assumption.
+Qed.
+
+Lemma insert_count_RBT :
+  forall (A : LinDec) (x y : A) (t : RBTree A),
+    count_RBT x (insert y t) = (if x =? y then S else id) (count_RBT x t).
+Proof.
+  intros. unfold insert.
+  rewrite makeBlack_count_RBT, ins_count_RBT. reflexivity.
+Qed.
+
+(** Properties of [toList]. *)
+
+Lemma toList_elem :
+  forall (A : Type) (x : A) (t : RBTree A),
+    In x (toList t) <-> elem x t.
+Proof.
+  split.
+    induction t; cbn; intros; try apply in_app_or in H; firstorder.
+      subst. firstorder.
+    induction 1; cbn; firstorder.
+Qed.
+
+Lemma toList_count_RBT :
+  forall (A : LinDec) (x : A) (t : RBTree A),
+    count_RBT x t = count A x (toList t).
+Proof.
+  induction t; cbn; dec.
+    rewrite count_app. cbn. rewrite IHt1, IHt2. dec.
+    rewrite count_app. cbn. rewrite IHt1, IHt2. dec.
+Qed.
+
+Lemma toList_sorted :
+  forall (A : LinDec) (t : RBTree A),
+    isBST t -> sorted A (toList t).
+Proof.
+  induction t as [| c l Hl v r Hr]; cbn; intros.
+    constructor.
+    inv H. apply sorted_app_all; auto.
+      case_eq (toList r); intros; subst; auto. constructor.
+        apply H6. rewrite <- toList_elem. rewrite H. cbn. auto.
+        rewrite <- H. auto.
+      intros. apply toList_elem in H. auto.
+Qed.
+
+(** Properties of [fromList]. *)
+
+Lemma fromList_elem :
+  forall (A : LinDec) (x : A) (l : list A),
+    elem x (fromList l) <-> In x l.
+Proof.
+  split.
+    induction l as [| h t]; cbn; intros.
+      inv H.
+      rewrite insert_elem in H. inv H.
+    induction l as [| h t]; cbn; intros.
+      inv H.
+      rewrite insert_elem. inv H.
+Qed.
+
+Lemma fromList_isBST :
+  forall (A : LinDec) (l : list A),
+    isBST (fromList l).
+Proof.
+  induction l as [| h t]; cbn.
+    constructor.
+    apply insert_isBST. assumption.
+Qed.
+
+Lemma fromList_count_RBT :
+  forall (A : LinDec) (x : A) (l : list A),
+    count_RBT x (fromList l) = count A x l.
+Proof.
+  induction l as [| h t]; cbn; dec;
+  rewrite insert_count_RBT, IHt; dec.
+Qed.
+
+(** Properties of [redblackSort]. *)
+
+Lemma redblackSort_sorted :
+  forall (A : LinDec) (l : list A),
+    sorted A (redblackSort A l).
+Proof.
+  intros. unfold redblackSort. apply toList_sorted, fromList_isBST.
+Qed.
+
+Lemma redblackSort_perm :
+  forall (A : LinDec) (l : list A),
+    perm A l (redblackSort A l).
+Proof.
+  unfold perm, redblackSort. intros.
+  rewrite <- toList_count_RBT, fromList_count_RBT. reflexivity.
+Qed.
